

MATH 325 HW 7

JALEN CHRYSOS

Problem 1: Let $\mathcal{U}(e, h, f)$ be an associative \mathbb{C} -algebra with generators e, h, f with relations

$$he - eh = 2e, \quad hf - fh = -2f, \quad ef - fe = h.$$

Let V be a $\mathcal{U}(e, h, f)$ -module and $v \in V$ a nonzero element such that $h(v) = \lambda v$ where $\lambda \in \mathbb{C}$.

- (a) Find an explicit formula for $h(f^i(v))$ as a function of λ .
- (b) Assume that $e(v) = 0$. Find explicit formulas for $e(f^i(v))$.
- (c) Show that if V is finite-dimensional then there is some nonzero $v \in V$ and nonnegative $d \in \mathbb{Z}$ such that $e(v) = 0$ and $h(v) = dv$.
- (d) Classify all simple finite-dimensional $\mathcal{U}(e, h, f)$ -modules up to isomorphism.

Proof. (a): We know $hf - fh = -2f$, so

$$hf(v) = (fh - 2f)(v) = (\lambda - 2)fv.$$

I claim that in general $h(f^i v) = (\lambda - 2i)f^i v$. This can be seen inductively:

$$\begin{aligned} hf^i v &= hf(f^{i-1} v) \\ &= (fh - 2f)(f^{i-1} v) \\ &= f(hf^{i-1} v) - 2f^i(v) \\ &= f(\lambda - 2(i-1))f^{i-1} v - 2f^i v \\ &= (\lambda - 2i)f^i v. \end{aligned}$$

Similarly $h(e^i v) = (\lambda + 2i)e^i v$.

(b): Because $ef - fe = h$,

$$ef(v) = (fe + h)(v) = f(0) + \lambda v = \lambda v.$$

For general i , we have $ef^i(v) = \lambda f^i v + ((i-1)\lambda - i(i+1))f^{i-1} v$ by induction:

$$\begin{aligned} ef^i(v) &= ef(f^{i-1} v) \\ &= (fe + h)(f^{i-1} v) \\ &= f(e f^{i-1} v) + h f^{i-1} v \\ &= (\lambda f^i v + ((i-2)\lambda - i(i-1))f^{i-1} v) + (\lambda - 2(i-1))f^{i-1} v \\ &= \lambda f^i v + ((i-1)\lambda - i(i+1))f^{i-1} v \end{aligned}$$

(c): Let v be any nonzero vector in V . By part (a), we see that $e^i v$ is an eigenvector of h for all i , and they all have different eigenvalues, so $e^i v = 0$ for all but finitely-many $i \in \mathbb{N}$. Thus let d be maximal such that $e^d v \neq 0$. Then $e(e^d v) = 0$ and $h(e^d v) = (\lambda + 2d)(e^d v)$.

We can view h with respect to the eigenbasis $v, ev, e^2 v, \dots, e^d v$ as the matrix

$$h = \begin{bmatrix} \lambda & 0 & 0 & \cdots & 0 \\ 0 & \lambda + 2 & 0 & \cdots & 0 \\ 0 & 0 & \lambda + 4 & \cdots & 0 \\ \vdots & \vdots & \vdots & \ddots & 0 \\ 0 & 0 & 0 & \cdots & \lambda + 2d \end{bmatrix}$$

1

and thus h has trace

$$\mathrm{tr}(h) = \sum_{i=0}^d \lambda + 2i = (d+1)\lambda + (d)(d+1) = (d+1)(\lambda + d).$$

But since $\mathrm{tr}(h) = \mathrm{tr}(ef - fe) = \mathrm{tr}(ef) - \mathrm{tr}(fe) = 0$, this implies $\lambda = -d$, and hence $h(e^d v) = de^d v$.

(d): Let V be a simple $\mathcal{U}(e, h, f)$ -module. By (c), there is some v with $e(v) = 0$ and $h(v) = dv$. By (a) and (b), the subspace $V' = \langle v, f(v), f^2(v), \dots \rangle$ is closed under multiplication by h and e , and clearly f as well, so V' is a submodule. Since V is simple and $V' \neq 0$ (as $v \neq 0$), $V' = V$.

As before, $f^i(v)$ is an h -eigenvector for all i , and they all have different eigenvalues, which implies that the nonzero $f^i(v)$ are all distinct and linearly independent. So because V is finite-dimensional, there must be some minimal n for which $f^n(v) = 0$. Then V has basis

$$V := \langle v, f v, f^2 v, \dots, f^{n-1} v \rangle$$

By (a) and (b), it's already determined how h, e, f act on this basis. So there is exactly one simple $\mathcal{U}(e, f, h)$ -module of dimension n up to isomorphism, for each n .

□

Problem 2:

(a) Check that the matrices

$$H = \begin{pmatrix} 1 & 0 \\ 0 & -1 \end{pmatrix}, \quad E = \begin{pmatrix} 0 & 1 \\ 0 & 0 \end{pmatrix}, \quad F = \begin{pmatrix} 0 & 0 \\ 1 & 0 \end{pmatrix}$$

form an \mathbb{R} -basis of the Lie algebra $\mathfrak{sl}_2(\mathbb{R})$ and that these matrices satisfy the relations in problem 1.

Proof. $\mathfrak{sl}_2(\mathbb{R})$ is exactly the matrices x such that $\det(e^{tx}) = e^{t \cdot \text{tr}(x)} = 1$ for all $t \in \mathbb{R}$, or equivalently $\text{tr}(x) = 0$. Thus, $\mathfrak{sl}_2(\mathbb{R})$ consists of the matrices

$$\begin{pmatrix} a & b \\ c & -a \end{pmatrix} = aH + bE + cF$$

for $a, b, c \in \mathbb{R}$. Thus E, F, H are a basis for $\mathfrak{sl}_2(\mathbb{R})$.

It is easy to check the three relations by just doing the matrix multiplications. In fact, we can check that $HE = E, EH = -E$, and $HF = -F, FH = F$, and

$$EF = \begin{bmatrix} 1 & 0 \\ 0 & 0 \end{bmatrix}, \quad FE = \begin{bmatrix} 0 & 0 \\ 0 & -1 \end{bmatrix}$$

The relations follow. □

Problem 3: Let $1_{ij} \in M_n(\mathbb{R})$ denote the matrices with 1 in the (i, j) place and 0 elsewhere.

- (a) Check that for any $i < j$, the matrices $e = 1_{ij}, h = 1_{ii} - 1_{jj}, f = 1_{ji}$ satisfy the relations in problem 1.
- (b) Let $\phi : M_n(\mathbb{R}) \rightarrow \text{End}_{\mathbb{C}}(V)$ be a Lie algebra representation, where $M_n(\mathbb{R}) = \text{Lie}(\text{GL}_n(\mathbb{R}))$ is viewed as a Lie algebra wrt the commutator and V is a finite-dimensional complex vector space. Prove (without using arguments from class) that there is a nonzero $v \in V$ and $\lambda_1, \dots, \lambda_n \in \mathbb{C}$ such that
- $\phi(1_{ii})(v) = \lambda_i v$ for all i .
 - $\phi(1_{ij})(v) = 0$ for all $i < j$.
 - $\lambda_i - \lambda_{i+1}$ is a nonnegative integer for all $1 \leq i \leq n-1$.

Proof. (a) Just as in problem 2, we can check that $he = e, eh = -e, hf = -f, fh = f$. And $ef = 1_{ii}, fe = 1_{jj}$, which shows $ef - fe = h$.

(b): Since $[1_{ii}, 1_{jj}] = 0$ for all i, j , the actions of $\phi(1_{ii})$ all pairwise commute as well. Thus if v is any eigenvector of $\phi(1_{ii})$ with eigenvalue λ_i , then

$$\phi(1_{jj})v = \lambda_i^{-1} \phi(1_{jj})\phi(1_{ii})v = \lambda_i^{-1} \phi(1_{ii})\phi(1_{jj})v$$

so $\phi(1_{jj})v$ is also an eigenvector of $\phi(1_{ii})$ with eigenvalue λ_i . Thus the $\phi(1_{ii})$ -eigenspace W corresponding to λ_i is both $\phi(1_{jj})$ -invariant.

Since $\phi(1_{jj})$ preserves W , there is at least some eigenvector $w \in W$ of $\phi(1_{jj})$ because \mathbb{C} is algebraically closed. Thus, the space of common eigenvectors between the two operators is non-trivial. In this way, one can continue inductively and show that the space of common eigenvectors between all the $\phi(1_{ii})$ is nontrivial, and thus contains some v with corresponding eigenvalues λ_i for $\phi(1_{ii})$.

Now for any $i < j$, $w := \phi(1_{ij})v$ is also an eigenvector for all $\phi(1_{kk})$, though with different eigenvalues;

$$\phi(1_{kk})w = \phi(1_{kk})\phi(1_{ij})v = (\phi(1_{ij})\phi(1_{kk}) + [\phi(1_{kk}), \phi(1_{ij})])v$$

in the case $k \notin \{i, j\}$, the commutator is 0, yielding

$$\phi(1_{kk})w = (\phi(1_{ij})\lambda_k)v = \lambda_k w$$

so the eigenvalue does not change. In the case $k = i$, the commutator is λ_{ij} , resulting in

$$\phi(1_{ii})w = (\phi(1_{ij})\lambda_i + \phi(1_{ij}))v = (\lambda_i + 1)w$$

so the eigenvalue increases by 1. In the case $k = j$, the commutator is $-\lambda_{ij}$, giving

$$\phi(1_{jj})w = (\phi(1_{ij})\lambda_j - \phi(1_{ij}))v = (\lambda_j - 1)w$$

so the eigenvalue decreases by 1. If we begin by maximizing the metric

$$n\lambda_1 + (n-1)\lambda_2 + \dots + \lambda_n$$

then replacing v by w would result in increasing this metric by

$$(n-i+1) - (n-j+i) = j-i$$

which would contradict maximality. Thus, w cannot exist, so $\phi(1_{ij})v = 0$.

To get the third condition, note that $\lambda_i - \lambda_{i+1}$ is the eigenvalue of v for $h = 1_{ii} - 1_{jj}$. By the same trace argument as in problem 1(c), we see that this eigenvalue must be a positive integer. \square

The group $\mathrm{GL}_2(k)$ acts on k^2 in the usual way. For $k = \mathbb{R}$ this action induces an action on $C^\infty(\mathbb{R}^2)$ by $g : p \mapsto g^*p$. For any $p \in C^\infty(\mathbb{R}^2)$ and $\chi \in \mathrm{Lie}(\mathrm{GL}_2(\mathbb{R})) = M_2(\mathbb{R})$, the Lie derivative $L_\chi(p)$ is a function on \mathbb{R}^2 defined by

$$(L_\chi(p))(x, y) = \left. \frac{d(e^{t\chi})^*(p) \cdot (x, y)}{dt} \right|_{t=0} = \left. \frac{d(p(e^{-t\chi}(x, y)))}{dt} \right|_{t=0}.$$

Problem 4: For $\chi = E, H, F$ as in problem 2, find an explicit formula for $L_\chi(p)$ in terms of the partials of the function p and check that the operators L_H, L_E, L_F satisfy relations in problem 1.

Proof. Let

$$e^{-t\chi} = \begin{bmatrix} a(t) & b(t) \\ c(t) & d(t) \end{bmatrix}.$$

Note that

$$\chi = \begin{bmatrix} -a'(0) & -b'(0) \\ -c'(0) & -d'(0) \end{bmatrix}.$$

We can calculate $L_\chi(p)$ as

$$\begin{aligned} L_\chi(p) &= \left. \frac{d(p(e^{-t\chi}(x, y)))}{dt} \right|_{t=0} \\ &= \left. \frac{dp(a(t)x + b(t)y, c(t)x + d(t)y)}{dt} \right|_{t=0} \\ &= (\partial_1 p)(a'(0)x + b'(0)y) + (\partial_2 p)(c'(0)x + d'(0)y) \\ &= (\partial_1 p) \cdot -\xi_1(x, y) + (\partial_2 p) \cdot -\xi_2(x, y). \end{aligned}$$

For $\xi \in \{H, E, F\}$ from the previous problem, this yields

$$L_H(p) = \partial_2 p \cdot y - \partial_1 p \cdot x, \quad L_E(p) = -\partial_1 p \cdot y, \quad L_F(p) = -\partial_2 p \cdot x.$$

Checking the relations from problem 1,

$$\begin{aligned} (L_H L_E - L_E L_H)(p) &= (\partial_2 L_E)y - (\partial_1 L_E)x - (\partial_1 L_H)y \\ &= (-\partial_1 p)y - 0 + (-\partial_1 p)y \\ &= -2(\partial_1 p)y = 2L_E(p) \end{aligned}$$

and similarly

$$\begin{aligned} (L_H L_F - L_F L_H)(p) &= (\partial_2 L_F)y - (\partial_1 L_F)x - (\partial_2 L_H)x \\ &= 0 - (-\partial_2 L_F)x - (-\partial_2 p)x \\ &= 2(\partial_2 p)x = -2L_F(p) \end{aligned}$$

and

$$\begin{aligned} (L_E L_F - L_F L_E)(p) &= (-\partial_1 L_F)y - (-\partial_2 L_E)x \\ &= (\partial_2 p)y - (\partial_1 p)x \\ &= L_H(p). \end{aligned}$$

□

Problem 5: Use problems 1 and 4 to prove that the representations $\mathrm{SL}_2(\mathbb{R}) \rightarrow \mathrm{GL}(P_d)$ are precisely the irreducible finite dimensional continuous representations of $\mathrm{SL}_2(\mathbb{R})$.

Proof. Let $\rho : \mathrm{SL}_2(\mathbb{R}) \rightarrow \mathrm{GL}(P_d)$ be the representation

$$\rho \begin{pmatrix} a & b \\ c & d \end{pmatrix} \cdot x^i y^j = (ax + by)^i (cx + dy)^j.$$

This is $d + 1$ dimensional. ρ is irreducible because $d\rho$ is, as we will show:

Note that

$$e^{tH} = I + tH + t^2 I/2 + t^3 H/6 + \cdots = \begin{bmatrix} e^t & 0 \\ 0 & e^{-t} \end{bmatrix}$$

and

$$e^{tE} = I + tE = \begin{bmatrix} 1 & t \\ 0 & 1 \end{bmatrix}, \quad e^{tF} = I + tF = \begin{bmatrix} 1 & 0 \\ t & 1 \end{bmatrix}.$$

So can calculate $d\rho$ on the basis H, E, F of $\mathfrak{sl}_2(\mathbb{R})$ as

$$\begin{aligned} d\rho(H)(x^i y^j) &= \partial_t \rho(e^{tH}) \cdot (x^i y^j)|_{t=0} \\ &= \partial_t ((e^t x)^i (e^{-t} y)^j)|_{t=0} \\ &= \partial_t e^{t(i-j)} x^i y^j|_{t=0} \\ &= (i - j)x^i y^j. \end{aligned}$$

For E , we have

$$\begin{aligned} d\rho(E)(x^i y^j) &= \partial_t \rho(e^{tE}) \cdot (x^i y^j)|_{t=0} \\ &= \partial_t (x + ty)^i (y)^j|_{t=0} \\ &= y \cdot i(x + ty)^{i-1} \cdot y^j|_{t=0} \\ &= ix^{i-1} y^{j+1}. \end{aligned}$$

Similarly,

$$\begin{aligned} d\rho(F)(x^i y^j) &= \partial_t \rho(e^{tF}) \cdot (x^i y^j)|_{t=0} \\ &= \partial_t (x)^i (y + tx)^j|_{t=0} \\ &= x^i \cdot j(y + tx)^{j-1} \cdot x|_{t=0} \\ &= jx^{i+1} y^{j-1}. \end{aligned}$$

The action of L_H, L_E, L_F on $C^\infty(\mathbb{R}^2)$ restricts to an action on P_d . It is easy to check, using the calculations from problem 4, that $d\rho(H)$ acts the same as L_H on P_d (up to sign), and similarly for $d\rho(E)$ and $d\rho(F)$. Thus, P_d is equivalent as a representation of $\mathbb{R}\langle L_H, L_E, L_F \rangle$ and as a representation of $\mathfrak{sl}_2(\mathbb{R})$, so the conclusion of problem 1 implies that there is exactly one n -dimensional irrep of $\mathfrak{sl}_2(\mathbb{R})$, which is P_{n-1} (one can see that the action on the basis $\{x^i y^j\}$ is the same).

Conversely, all irreps of $\mathrm{SL}_2(\mathbb{R})$ are of this form. This follows from the classification theorem which says that there is exactly one irrep with a given highest weight, which in this case is $(d, d - 2, d - 4, \dots, -d)$. \square

Problem 6:

- (a) Show that the group SU_2 of unitary 2×2 matrices with determinant 1 is formed by the matrices

$$\left\{ g = \begin{pmatrix} a & b \\ -\bar{b} & \bar{a} \end{pmatrix} \mid a, b \in \mathbb{C}, |a|^2 + |b|^2 = 1 \right\}.$$

- (b) Check that the following matrices form an \mathbb{R} -basis of the Lie algebra $\mathfrak{su}_2 = \text{Lie}(SU_2) \subset M_2(\mathbb{C})$:

$$I_1 = \begin{pmatrix} i & 0 \\ 0 & -i \end{pmatrix}, \quad I_2 = \begin{pmatrix} 0 & 1 \\ -1 & 0 \end{pmatrix}, \quad I_3 = \begin{pmatrix} 0 & i \\ i & 0 \end{pmatrix}$$

- (c) Find $[I_i, I_j]$ for $i, j \in \{1, 2, 3\}$ and express I_i in terms of H, F, E .

Proof. (a): If

$$g = \begin{pmatrix} a & b \\ c & d \end{pmatrix} \in SU_2$$

then being unitary implies that $|a|^2 + |b|^2 = 1$ and $a\bar{c} + b\bar{d} = 0$, so $\bar{d}/a = -\bar{c}/b$. If this ratio is $x \in \mathbb{C}$, then we have $d = \bar{a}x$ and $c = -\bar{b}x$. Using the fact that g has determinant 1,

$$1 = ad - bc = a(\bar{a}x) - b(-\bar{b}x) = (|a|^2 + |b|^2)x \implies x = 1$$

so

$$g = \begin{pmatrix} a & b \\ -\bar{b} & \bar{a} \end{pmatrix}$$

as desired. Moreover, for any $a, b \in \mathbb{C}$ such that $|a|^2 + |b|^2 = 1$, this g is clearly in SU_2 .

(b): We showed in a previous homework that \mathfrak{u}_2 consists of the skew-hermitian matrices, and that \mathfrak{sl}_2 is the trace 0 matrices. Thus, \mathfrak{su}_2 is the intersection of these:

$$\begin{pmatrix} ir & s + it \\ -s + it & -ir \end{pmatrix}$$

where $r, s, t \in \mathbb{R}$. So over \mathbb{R} , it is clearly generated by I_1, I_2, I_3 .

(c): Note that $I_1 = iH$, $I_2 = E - F$, and $I_3 = i(E + F)$. This gives

$$[I_1, I_2] = iH(E - F) - (E - F)iH = i(HE - HF - EH + FH) = i(2E + 2F) = 2I_3.$$

$$[I_2, I_3] = (E - F)i(E + F) - i(E + F)(E - F) = 2i(EF - FE) = 2iH = 2I_1.$$

$$[I_3, I_1] = i(E + F)iH - iHi(E + F) = HE + HF - EH - FH = 2E - 2F = 2I_2.$$

□

Problem 7:

- (a) Classify irreducible representations of \mathfrak{su}_2 in finite-dimensional complex vector spaces up to isomorphism.
- (b) Let $g_d : SU_2 \rightarrow GL(P_d)$ be the representation of SU_2 in the vector space P_d . Show that the representations g_d are precisely the irreducible finite-dimensional continuous representations of SU_2 .

Proof. (a): As shown in problem 6, $I_1 = iH, I_2 = E - F, I_3 = i(E + F)$. It follows that $H, E, F \in \mathfrak{su}_2$ as linear combinations of I_1, I_2, I_3 :

$$H = -iI_1, \quad E = \frac{1}{2}(I_2 - iI_3), \quad F = \frac{1}{2}(-I_2 - iI_3)$$

In fact, \mathfrak{su}_2 is a \mathbb{C} -algebra generated by H, E, F , since they generate I_1, I_2, I_3 which in turn generate \mathfrak{su}_2 . Thus, the conclusion in problem 1 (d) applies, showing that there is exactly one n -dimensional irrep for each n , up to isomorphism.

(b): First, g_d is irreducible because dg_d is, which follows from problem 1 if we check that $dg_d(H)$ (and E, F) have the same action on the basis elements of $x^i y^j$ as dictated in problem 1. And unlike in problem 5, the converse also holds automatically because SU_2 is simply connected, so because dg_d is the unique irrep of \mathfrak{su}_2 , g_d must be the unique irrep of SU_2 as well. \square

Problem 8: Let $\text{Ad} : SU_2 \rightarrow \text{GL}(\mathfrak{su}_2)$ be the representation of SU_2 that sends $g \in SU_2$ to $\text{Ad } g : \mathfrak{su}_2 \rightarrow \mathfrak{su}_2$, where $\text{Ad } g : x \mapsto gxg^{-1}$. Let $d(\text{Ad}) : \mathfrak{su}_2 \rightarrow \text{End}_{\mathbb{R}}(\mathfrak{su}_2) = \text{Lie}(\text{GL}(\mathfrak{su}_2))$ be the differential of the representation Ad .

- (a) Show that $\ker(\text{Ad}) = \pm \text{id}$ and that $d(\text{Ad})$ is injective.
- (b) Construct a surjective morphism of Lie groups $SU_2 \rightarrow \text{SO}_3(\mathbb{R})$ with kernel $\pm \text{id}$. That is, construct an isomorphism $\text{SO}_3(\mathbb{R}) \cong SU_2 / \{\pm \text{id}\}$.

Proof. (a): If $\text{Ad}(g) = \text{id}$, then $gxg^{-1} = x$ for all $x \in \mathfrak{su}_2$, or equivalently for each of the three basis matrices. Let

$$g = \begin{pmatrix} a & b \\ c & d \end{pmatrix}.$$

If g commutes with I_1 then it follows that $b = c = 0$. If g commutes with I_2 then it follows that $a = d$. Finally, because $g \in SU_2$ to begin with, $ad - bc = 1$, hence $a^2 = 1$. Thus g is either id or $-\text{id}$, as expected.

To show that $d(\text{Ad})$ is injective, we have by proposition 9.6.2(2) that

$$\ker(d \text{Ad}) = \text{Lie}(\ker(\text{Ad})) = \text{Lie}(\pm \text{id}) = 0$$

noting that $e^{tx} = \pm \text{id}$ for all $t \in \mathbb{R}$ implies $x = 0$, as \exp is invertible near 0.

(b): We'll show that Ad is such a morphism by showing that it is surjective onto $\text{SO}_3(\mathbb{R})$.

The basis I_1, I_2, I_3 of \mathfrak{su}_2 is orthonormal with inner product $\langle a, b \rangle = -\frac{1}{2} \text{tr}(ab)$. Any $\text{Ad}(g)$ preserves this inner product, as

$$-\frac{1}{2} \text{tr}(\text{Ad } g(x) \text{Ad } g(y)) = -\frac{1}{2} \text{tr}(gxyg^{-1}) = -\frac{1}{2} \text{tr}(xy)$$

because trace is invariant under conjugation. Thus, we see that $\text{Ad } g$ is an orthogonal transformation on the 3-dimensional basis of \mathfrak{su}_2 , so the image of Ad lies within $\text{O}_3(\mathbb{R})$. Thus the image of $d \text{Ad}$ lies within $\text{Lie}(\text{O}_3(\mathbb{R}))$, which we know to be the skew-symmetric matrices in $M_3(\mathbb{R})$, a 3-dimensional subspace:

$$\mathfrak{o}_3(\mathbb{R}) = \left\{ \begin{pmatrix} 0 & a & b \\ -a & 0 & c \\ -b & -c & 0 \end{pmatrix} \mid a, b, c \in \mathbb{R} \right\}$$

Then $d \text{Ad} : \mathfrak{su}_2 \rightarrow \mathfrak{o}_3$ is a map $\mathbb{R}^3 \rightarrow \mathbb{R}^3$. We know from part (a) that it is injective, so it is also surjective. And note that $\mathfrak{o}_3(\mathbb{R}) = \mathfrak{so}_3(\mathbb{R})$, since $\det(e^{tx}) = 1 \iff \text{tr}(x) = 0$ is already true in $\mathfrak{o}_3(\mathbb{R})$. So in fact $d \text{Ad}$ is bijective on $\mathfrak{so}_3(\mathbb{R})$.

Ad cannot be surjective onto $\text{O}_3(\mathbb{R})$, as SU_2 is connected and Ad is continuous, so $\text{im}(\text{Ad})$ must be connected as well. This implies that $\text{im}(\text{Ad})$ is contained in the connected component of 1, which is $\text{SO}_3(\mathbb{R})$ (we showed this to be connected in previous homework). And because $d \text{Ad}$ is surjective on $\mathfrak{so}_3(\mathbb{R})$, Ad must be surjective on $\text{SO}_3(\mathbb{R})$ as well. \square

Problem 9:

- (a) Prove that any continuous irreducible representation of the group $\mathrm{SO}_3(\mathbb{R})$ has odd dimension. Moreover, for every odd integer $2m + 1$, there is exactly one continuous irreducible representation of dimension $2m + 1$.
- (b) Prove theorem 2.1.2(2), which says that any continuous finite-dimensional representation of $\mathrm{SO}_3(\mathbb{R})$ is isomorphic to the representation H_d for some $d \geq 0$.

Proof. (a): As shown in problem 8, $\mathrm{SO}_3(\mathbb{R})$ is isomorphic to $SU_2/\{\pm \mathrm{id}\}$ via Ad. Thus, representations of $\mathrm{SO}_3(\mathbb{R})$ map to representations of SU_2 by just having $-\mathrm{id}$ act trivially. Because there is a unique representation of SU_2 in each dimension, there can be a representation of SO_3 iff the induced representation of SU_2 is g_p ; that is, if $-\mathrm{id}$ acts trivially. In g_d , $-\mathrm{id}$ acts as scaling by $(-1)^d$ on P_d . This is trivial iff d is even, hence when P_d has odd dimension.

(b): Recall that $P_d = RP_{d-2} \oplus H_d$, so

$$\dim(H_d) = \dim(P_d) - \dim(P_{d-2}) = \binom{d}{2} - \binom{d-2}{2} = 2d + 1$$

thus H_d is the unique continuous representation of $\mathrm{SO}_3(\mathbb{R})$ in dimension $2d + 1$. □